Sorted equivalences

BTree.thy
@@ -15,9 +15,6 @@ text "General structure:  nat values in the leafs and nat/tree node internal nod
 
 datatype 'a btree = Leaf | Node "('a btree * 'a) list"
 
-definition "btree_of_pair = fst"
-definition "sep_of_pair = snd"
-
 fun inorder :: "'a btree \<Rightarrow> 'a list" where
 "inorder Leaf = []" |
 "inorder (Node kvs) = (foldr (@) (map (\<lambda> (sub, sep). inorder sub @ [sep]) kvs) [])" 
@@ -46,26 +43,22 @@ value "inorder (Node [(Leaf, (1::nat)), (Node [(Leaf, 1), (Leaf, 10)], 10), (Lea
 fun subtrees where "subtrees xs = (map fst xs)"
 fun seperators where "seperators xs = (map snd xs)"
 
-definition btree_set:: "'a btree \<Rightarrow> 'a set" where 
-  "btree_set = set \<circ> inorder"
+definition set_btree_inorder:: "'a btree \<Rightarrow> 'a set" where 
+  "set_btree_inorder = set \<circ> inorder"
 
 thm btree.simps
-(* TODO use set_btree instead *)
-fun btree_set_alt:: "'a btree \<Rightarrow> 'a set" where
-"btree_set_alt Leaf = {}" |
-"btree_set_alt (Node t) = set (seperators t) \<union> \<Union> (set (map (btree_set_alt) (subtrees t)))"
-
-
+find_theorems set_btree
+value "set_btree (Node [(Leaf, 1::nat)])"
 
 lemma append_foldr_set: "set (foldr (@) xs []) = \<Union> (set (map set xs))"
   apply(induction xs)
    apply(auto)
   done
 
-lemma btree_set_set_def: "btree_set t = btree_set_alt t"
+lemma set_btree_inorder_set_btree: "set_btree_inorder t = set_btree t"
   apply(induction t)
-   apply(auto simp add: btree_set_def append_foldr_set)
-  by (metis image_eqI snd_conv)
+   apply(auto simp add: set_btree_inorder_def append_foldr_set)
+  done
 
 fun bal:: "'a btree \<Rightarrow> bool" where
 "bal Leaf = True" |
@@ -79,44 +72,16 @@ fun k_spread:: "nat \<Rightarrow> 'a btree \<Rightarrow> bool" where
 "k_spread k (Node t) = ((length t \<ge> k \<and> length t \<le> 2*k+1) \<and> (\<forall>sub \<in> set (subtrees t). k_spread k sub))"
 
 
-(*TODO: at some point this better be replaced with something binary search like *)
-(* split *)
-fun btree_list_choose_help:: "(('a::linorder) btree\<times>'a) list \<Rightarrow> 'a \<Rightarrow> ('a btree\<times>'a) list \<Rightarrow>  (('a btree\<times>'a) list \<times> ('a btree\<times>'a) list)" where
-"btree_list_choose_help [] x prev = (prev, [])" |
-"btree_list_choose_help ((sub, sep)#xs) x prev = (if sep < x then btree_list_choose_help xs x (prev @ [(sub, sep)]) else (prev, (sub,sep)#xs))"
-
-fun btree_list_choose:: "(('a::linorder) btree\<times>'a) list \<Rightarrow> 'a \<Rightarrow> (('a btree\<times>'a) list \<times> ('a btree\<times>'a) list)" where
-"btree_list_choose xs x = btree_list_choose_help xs x []"
-
-
-lemma [termination_simp]:"(x, (a, b) # x22) = btree_list_choose_help t y xs \<Longrightarrow>
-       y \<noteq> b \<Longrightarrow> size a < Suc (size_list (\<lambda>x. Suc (size (fst x))) t)"
-  apply(induction t y xs arbitrary: a b x x22 rule: btree_list_choose_help.induct)
-  apply(simp_all)
-  by (metis add_Suc_right less_SucI less_add_Suc1 list.inject old.prod.inject trans_less_add2)
-
-fun isin:: "('a::linorder) btree \<Rightarrow> 'a \<Rightarrow> bool" where
- "isin (Leaf) y = False" |
- "isin (Node t) y = (case btree_list_choose t y of (_,r) \<Rightarrow> (case r of [] \<Rightarrow> False | (sub,sep)#xs \<Rightarrow> (if y = sep then True else isin sub y)))"
-
-
-value "btree_set (Node [(Leaf, (0::nat)), (Node [(Leaf, 1), (Leaf, 10)], 12), (Leaf, 30), (Leaf, 100)])"
+value "set_btree_inorder (Node [(Leaf, (0::nat)), (Node [(Leaf, 1), (Leaf, 10)], 12), (Leaf, 30), (Leaf, 100)])"
 value "height (Node [(Leaf, (0::nat)), (Node [(Leaf, 1), (Leaf, 10)], 12), (Leaf, 30), (Leaf, 100)])"
 (* a bit weird *)
 value "size (Node [(Leaf, (0::nat)), (Node [(Leaf, 1), (Leaf, 10)], 12), (Leaf, 30), (Leaf, 100)])"
 
 
-lemma child_subset: "p \<in> set t \<Longrightarrow> btree_set (fst p) \<subseteq> btree_set (Node t)"
+lemma child_subset: "p \<in> set t \<Longrightarrow> set_btree (fst p) \<subseteq> set_btree (Node t)"
   apply(induction p arbitrary: t)
-   apply(auto simp add: btree_set_def append_foldr_set)
+   apply(auto)
   done
-
-
-lemma some_child_pair: 
- "btree_list_choose_help t y xs = (l,(sub,sep)#ts) \<Longrightarrow> (sub,sep) \<in> set t"
-  apply(induction t y xs arbitrary: l sub sep ts rule: btree_list_choose_help.induct)
-   apply(simp_all)
-  by (metis Pair_inject list.inject)
 
 lemma some_child_sub: 
   assumes "(sub,sep) \<in> set t"
@@ -124,291 +89,100 @@ lemma some_child_sub:
   and "sep \<in> set (seperators t)"
   using assms by force+ 
 
-lemma some_child_sm: "btree_list_choose_help t y xs = (l,(sub,sep)#ts) \<Longrightarrow> y \<le> sep"
-  apply(induction t y xs arbitrary: l sub sep ts rule: btree_list_choose_help.induct)
-  apply(simp_all)
-  by (metis Pair_inject le_less_linear list.inject)
-
-
-lemma isin_true_not_empty_r: "\<lbrakk>isin (Node t) y; btree_list_choose_help t y [] = (l, r)\<rbrakk> \<Longrightarrow> r \<noteq> []"
-  unfolding isin.simps by auto
-
-
-lemma isin_implied_in_set: "isin n y \<Longrightarrow> y \<in> btree_set n"
-proof(induction n y rule: isin.induct)
-  case (2 t y)
-  then obtain l r where 21: "btree_list_choose_help t y [] = (l,r)" by auto
-  then have "r \<noteq> []" using isin_true_not_empty_r 2 by auto
-  then obtain sub sep xs where 22: "r = (sub,sep)#xs" by (cases r) auto
-  then have "y = sep \<or> y \<noteq> sep" using 21 22 by blast
-  then show ?case
-  proof
-    assume "y = sep"
-    then have "y \<in> set (seperators t)" using some_child_sub(2) some_child_pair 2 21 22
-      by metis
-    then show "y \<in> btree_set (Node t)" by (simp add: btree_set_set_def)
-  next
-    assume "y \<noteq> sep"
-    then have "y \<in> btree_set sub" unfolding btree_list_choose.simps using 2 21 22 by auto
-    then show "y \<in> btree_set (Node t)"
-      using "21" "22" child_subset some_child_pair by fastforce
-  qed
-qed simp
-
 (* idea: make sorted_list a sorted_wrt *)
 find_theorems sorted_wrt
 thm sorted_wrt_append
 
 fun sub_sep_sm where
  "sub_sep_sm (sub_l, sep_l) (sub_r, sep_r) =
-  ((sep_l < sep_r) \<and> (\<forall>x \<in> btree_set sub_r. sep_l < x))"
+  ((sep_l < sep_r) \<and> (\<forall>x \<in> set_btree sub_r. sep_l < x))"
 
 fun sub_sep_cons where
-"sub_sep_cons (sub, sep) = (\<forall>x \<in> btree_set sub. x < sep)"
+"sub_sep_cons (sub, sep) = (\<forall>x \<in> set_btree sub. x < sep)"
 
 lemma sorted_wrt_list_sorted: "sorted_wrt sub_sep_sm xs \<Longrightarrow> sorted (seperators xs)"
   apply(induction xs) 
    apply (auto simp add: sorted_wrt_Cons)
   done
 
-lemma sorted_wrt_sorted_left: "sorted_wrt sub_sep_sm ((sub, sep)#xs) \<Longrightarrow> t \<in> set (subtrees xs) \<Longrightarrow> \<forall>x \<in> btree_set t. x > sep"
+lemma sorted_wrt_sorted_left: "sorted_wrt sub_sep_sm ((sub, sep)#xs) \<Longrightarrow> t \<in> set (subtrees xs) \<Longrightarrow> \<forall>x \<in> set_btree t. x > sep"
   apply(induction xs) 
    apply (auto simp add: sorted_wrt_Cons)
   done
 
+
 (* the below is independent of the inter-pair sorting *)
-lemma sorted_wrt_sorted_right: "\<forall>x \<in> set xs. sub_sep_cons x \<Longrightarrow> (t, sep) \<in> set xs \<Longrightarrow> \<forall>x \<in> btree_set t. x < sep"
+lemma sorted_wrt_sorted_right: "\<forall>x \<in> set xs. sub_sep_cons x \<Longrightarrow> (t, sep) \<in> set xs \<Longrightarrow> \<forall>x \<in> set_btree t. x < sep"
   by auto
 
-fun sorted_alt2 where
-"sorted_alt2 Leaf = True" |
-"sorted_alt2 (Node xs) = (sorted_wrt sub_sep_sm xs \<and> (\<forall>x \<in> set xs. sub_sep_cons x) \<and> (\<forall>sub \<in> set (subtrees xs). sorted_alt2 sub))"
+fun sorted_alt where
+"sorted_alt Leaf = True" |
+"sorted_alt (Node xs) = (sorted_wrt sub_sep_sm xs \<and> (\<forall>x \<in> set xs. sub_sep_cons x) \<and> (\<forall>sub \<in> set (subtrees xs). sorted_alt sub))"
 
-value "sorted_alt (Node [(Node [(Node [], a\<^sub>1)], a\<^sub>2)])"
 value "sorted (inorder (Node [(Node [(Node [], a\<^sub>1)], a\<^sub>2)]))"
-value "sorted_alt2 (Node [(Node [(Node [], a\<^sub>1)], a\<^sub>2)])"
+value "sorted_alt (Node [(Node [(Node [], a\<^sub>1)], a\<^sub>2)])"
 
-lemma "(sorted (inorder sub) \<and> (\<forall>x \<in> btree_set sub. x < sep)) = sorted((inorder sub) @ [sep])"
-  unfolding btree_set_def using sorted_snoc_iff
+lemma sorted_pair_list: "(sorted (inorder sub) \<and> (\<forall>x \<in> set_btree_inorder sub. x < sep)) = sorted((inorder sub) @ [sep])"
+  unfolding set_btree_inorder_def using sorted_snoc_iff
   by auto
 
 
-(* idea: we show that if any element is in the btree_set of a tree, then it must be in the list or in the subtree given by btree_list_choose,
+(* idea: we show that if any element is in the set_btree_inorder of a tree, then it must be in the list or in the subtree given by btree_list_choose,
 show the latter by case distinction on the compare of btree_list *)
 
-lemma btree_set_alt_induct: "x \<in> btree_set_alt (Node xs) \<Longrightarrow> x \<in> set (seperators xs) \<or> (\<exists>sub \<in> set (subtrees xs). x \<in> btree_set_alt sub)"
+lemma set_btree_induct: "x \<in> set_btree (Node xs) \<Longrightarrow> x \<in> set (seperators xs) \<or> (\<exists>sub \<in> set (subtrees xs). x \<in> set_btree sub)"
   apply(induction xs)
    apply(auto)
   done
 
 find_theorems sorted_wrt map
 
-lemma btree_list_choose_append: "btree_list_choose_help xs p ys = (l,r) \<Longrightarrow> l@r = ys@xs"
-  apply(induction xs p ys arbitrary: l r rule: btree_list_choose_help.induct)
-   apply(simp_all)
-  apply(metis Pair_inject)
-  done
-
-lemma btree_list_choose_sm: "\<lbrakk>btree_list_choose_help xs p ys = (l,r); sorted (seperators (ys@xs)); \<forall>sep \<in> set (seperators ys). p > sep\<rbrakk> \<Longrightarrow> \<forall>sep \<in> set (seperators l). p > sep"
-  apply(induction xs p ys arbitrary: l r rule: btree_list_choose_help.induct)
-   apply(simp_all)
-  by (metis prod.inject)+
-
-value "btree_list_choose [(Leaf, 2)] (1::nat)"
-find_theorems sorted_wrt "(@)"
-
-lemma btree_list_choose_gr: "\<lbrakk>btree_list_choose_help xs p ys = (l,r); sorted (seperators (ys@xs)); \<forall>(sub,sep) \<in> set ys. p > sep\<rbrakk> \<Longrightarrow> 
-(case r of [] \<Rightarrow> True | ((psub, psep)#rs) \<Rightarrow> p \<le> psep \<and> (\<forall>sep \<in> set (seperators rs). p < sep))"
-proof(induction xs p ys arbitrary: l r rule: btree_list_choose_help.induct)
-  case (2 sub sep xs x prev)
-  then obtain l r where btree_choose_lr: "btree_list_choose_help ((sub, sep)#xs) x prev = (l,r)" by auto
-  then show ?case
-  using 2 proof (cases r)
-  case (Cons a list)
-  then obtain psub psep where a_head: "a = (psub, psep)" by (cases a)
-  then have 21: "x \<le> psep" using  btree_choose_lr Cons some_child_sm by blast
-  also from 2 Cons have "\<forall>(sub,sep) \<in> set list. x < sep"
-  proof -
-    have "sorted (seperators (l@r))" using btree_list_choose_append btree_choose_lr
-      by (metis "2.prems"(2))
-    then have "sorted ((seperators l)@(seperators r))" by simp
-    then have "sorted (seperators r)" using sorted_wrt_append by auto
-    then have "sorted (seperators ((psub,psep)#list))" using a_head Cons by blast
-    then have "sorted (psep#(seperators list))" by auto
-    then have "\<forall>(sub,sep) \<in> set list. sep > psep"
-      by (metis case_prodI2 some_child_sub(2) sorted_wrt_Cons)
-    then show ?thesis
-      using calculation by auto
-  qed
-    ultimately show ?thesis
-      using "2.prems"(1) \<open>a = (psub, psep)\<close> btree_choose_lr local.Cons by auto 
-  qed simp
-qed simp
-
-    
-
-
-
-(* idea: our only requirement for btree_list_choose are the following two*)
-(*TODO make btree_list_choose return the matching pair and the list left and right as well*)
-lemma btree_list_choose_req:
-  assumes  "btree_list_choose xs p = (l,r)"
-    and "sorted (seperators xs)"
-  shows "l @ r = xs"
-  and "\<forall>sep \<in> set (seperators l). p > sep"
-  and "(case r of [] \<Rightarrow> True | ((psub, psep)#rs) \<Rightarrow> (p \<le> psep \<and> (\<forall>sep \<in> set (seperators rs). p < sep)))"
-proof - 
-  show "l@r = xs"
-    using assms(1) btree_list_choose_append by force
-next
-  show "\<forall>sep \<in> set (seperators l). p > sep" using assms btree_list_choose_sm by force
-next
-  show "(case r of [] \<Rightarrow> True | ((psub, psep)#rs) \<Rightarrow> (p \<le> psep \<and> (\<forall>sep \<in> set (seperators rs). p < sep)))"
-    using assms btree_list_choose_gr by force
-qed
-
-  
-
-(* from the above simple requirements, we may follow the isin requirements (hopefully) *)
-lemma btree_list_choose_seperator_match:
-  assumes "sorted (seperators xs)" 
-    and "y \<in> set (seperators xs)" 
-    and "btree_list_choose xs y = (l,r)"
-  shows "snd (hd r) = y"
-  and "r \<noteq> []"
-proof -
-  have "y \<in> set (seperators (l@r))" using btree_list_choose_req(1) assms by blast
-  also have "y \<notin> set (seperators l)"
-    using assms(1) assms(3) btree_list_choose_req(2) by blast
-  ultimately have "y \<in> set (seperators r)"
-    by simp
-  then show "snd (hd r) = y"
-  proof (cases r)
-    case (Cons a list)
-    then obtain psub psep where a_split: "a = (psub, psep)" by (cases a)
-    then have "(\<forall>x \<in> set (seperators list). y < x)" using  btree_list_choose_req(3)[of xs y l r] assms Cons by auto
-    then have "y \<notin> set (seperators list)" by auto
-    then have "y = psep" using \<open>y \<in> set (seperators r)\<close> Cons a_split by simp
-    then show ?thesis using Cons a_split by auto
-  qed simp
-  from \<open>y \<in> set (seperators r)\<close> show "r \<noteq> []" by auto
-qed
-
-thm sorted_wrt_sorted_left
-
-lemma btree_list_choose_subtree_match:
-  assumes "\<exists>sub \<in> set (subtrees xs). y \<in> btree_set sub"
-  assumes "sorted_wrt sub_sep_sm xs"
-  assumes "\<forall>x \<in> set xs. sub_sep_cons x"
-  assumes "btree_list_choose xs y = (l,r)"
-  shows "y \<in> btree_set (fst (hd r))"
-  and "r \<noteq> []"
-proof -
-  have "\<forall> (sub,sep) \<in> set l. y > sep"
-    using assms(2) assms(4) btree_list_choose_req(2) sorted_wrt_list_sorted by fastforce
-  then have "\<forall> (sub, sep) \<in> set l. y \<notin> btree_set sub"
-    by (metis (no_types, lifting) Un_iff assms(2) assms(3) assms(4) btree_list_choose_req(1) btree_list_choose_req(2) btree_set_set_def case_prodI2 less_asym' set_append some_child_sub(2) sorted_wrt_list_sorted sub_sep_cons.simps)
-  moreover have "\<exists>sub \<in> set (subtrees (l@r)). y \<in> btree_set sub"
-    using assms(1) assms(2) assms(4) btree_list_choose_req(1) sorted_wrt_list_sorted by blast
-  ultimately have "\<exists>sub \<in> set (subtrees r). y \<in> btree_set sub" by auto
-  then show "y \<in> btree_set (fst (hd r))"
-  proof (cases r)
-    case (Cons a list)
-    then obtain psub psep where a_split: "a = (psub, psep)" by (cases a)
-    then have "y \<le> psep" 
-      using  btree_list_choose_req(3)[of xs y l r] assms Cons sorted_wrt_list_sorted by fastforce
-    moreover have "\<forall>t \<in> set (subtrees list). \<forall>x \<in> btree_set t. psep < x"
-      using sorted_wrt_sorted_left a_split assms(2) assms(4) btree_list_choose_req(1) local.Cons sorted_wrt_append sorted_wrt_list_sorted by blast
-    ultimately have "\<forall>t \<in> set (subtrees list). y \<notin> btree_set t"
-      using leD by blast
-    then have "y \<in> btree_set psub"
-      using \<open>\<exists>sub\<in>set (subtrees r). y \<in> btree_set sub\<close> a_split local.Cons by auto
-    then show ?thesis
-      by (simp add: a_split local.Cons)
-  qed simp
-  from \<open>\<exists>sub \<in> set (subtrees r). y \<in> btree_set sub\<close> show "r \<noteq> []" by auto
-qed
-
-thm btree_list_choose_subtree_match
-
-lemma isin_set: "sorted_alt2 t \<Longrightarrow> x \<in> btree_set t \<Longrightarrow> isin t x"
-proof (induction t x rule: isin.induct)
-  case (2 xs y)
-    obtain l r where choose_split: "btree_list_choose xs y = (l,r)"
-      by fastforce
-  from 2 have "y \<in> set (seperators xs) \<or> (\<exists>sub \<in> set (subtrees xs). y \<in> btree_set sub)"
-    using btree_set_alt_induct by (simp add: btree_set_set_def)
-  then show ?case
-  proof
-    assume asm: "y \<in> set (seperators xs)"
-    then have "snd (hd r) = y" "r \<noteq> []" using choose_split btree_list_choose_seperator_match asm 2 sorted_wrt_list_sorted
-      by (metis sorted_alt2.simps(2))+
-    then show "BTree.isin (Node xs) y" unfolding isin.simps
-      using choose_split by (cases r) auto
-  next
-    assume asms: "(\<exists>sub \<in> set (subtrees xs). y \<in> btree_set sub)"
-    then have "y \<in> btree_set (fst (hd r))" "r \<noteq> []"
-      using choose_split btree_list_choose_subtree_match
-      by (metis "2.prems"(1) sorted_alt2.simps(2))+
-    moreover have "fst (hd r) \<in> set (subtrees xs)"
-      by (metis (no_types, lifting) btree_list_choose.elims calculation(2) choose_split eq_fst_iff list.sel(1) list.set_cases list.set_sel(1) some_child_pair some_child_sub(1))
-    ultimately show "BTree.isin (Node xs) y" using 2 choose_split
-      unfolding isin.simps by (cases r) (fastforce)+
-  qed
-qed (auto simp add: btree_set_set_def)
-
-lemma "sorted_alt2 t \<Longrightarrow> isin t y = (y \<in> btree_set t)"
-  using BTree.isin_set btree_set_set_def isin_implied_in_set by fastforce
-
-lemma "\<lbrakk>\<forall>y \<in> set ys. \<forall>x \<in> set xs. y < x; sorted ys; sorted xs\<rbrakk> \<Longrightarrow> sorted (ys@xs)"
-  using sorted_wrt_append by blast
-
 
 find_theorems sorted_wrt "(@)"
 find_theorems sorted_wrt "(#)"
 thm sorted_wrt_append
 
-lemma "sorted_alt2 t \<Longrightarrow> sorted (inorder t)"
+lemma sorted_alt_sorted: "sorted_alt t \<Longrightarrow> sorted (inorder t)"
 proof(induction t)
   case (Node xs)
-  then have "\<lbrakk>sorted_alt2 (Node xs)\<rbrakk> \<Longrightarrow> sorted (inorder (Node xs))"
+  then have "\<lbrakk>sorted_alt (Node xs)\<rbrakk> \<Longrightarrow> sorted (inorder (Node xs))"
   proof (induction xs)
     case (Cons a list)
     then have Cons_help: 
       "sorted_wrt sub_sep_sm list" 
       "\<forall>x \<in> set list. sub_sep_cons x"
-      "\<forall>sub \<in> set (subtrees list). sorted_alt2 sub"
+      "\<forall>sub \<in> set (subtrees list). sorted_alt sub"
       by (simp add: sorted_wrt_Cons)+
-    then have "sorted_alt2 (Node list)" using Cons
+    then have "sorted_alt (Node list)" using Cons
       by simp
     then have Cons_sorted: "sorted (inorder (Node list))"
       using Cons.IH Cons.prems(2) by auto
 
     from Cons obtain sub sep where pair_a: "a = (sub,sep)" by (cases a) simp
-    then have "sorted_alt2 sub" using Node Cons
+    then have "sorted_alt sub" using Node Cons
       by simp
     then have "sorted (inorder sub)" using Node Cons pair_a
       by force
 
     from pair_a have "\<forall>x \<in> set (seperators list). sep < x"
       using sorted_wrt_Cons sorted_wrt_list_sorted Cons_help
-      by (metis (no_types, lifting) Cons.prems(1) list.simps(9) seperators.simps snd_conv sorted_alt2.simps(2))
-    also from pair_a Cons have "\<forall>t \<in> set (subtrees list). (\<forall>x \<in> btree_set t. sep < x)"
-      using sorted_alt2.simps(2) sorted_wrt_sorted_left by blast
-    ultimately have "\<forall>x \<in> btree_set_alt (Node list). sep < x"
-      using btree_set_set_def by fastforce
-    then have "\<forall>x \<in> btree_set (Node list). sep < x"
-      by (simp add: btree_set_set_def)
+      by (metis (no_types, lifting) Cons.prems(1) list.simps(9) seperators.simps snd_conv sorted_alt.simps(2))
+    also from pair_a Cons have "\<forall>t \<in> set (subtrees list). (\<forall>x \<in> set_btree t. sep < x)"
+      using sorted_alt.simps(2) sorted_wrt_sorted_left by blast
+    ultimately have "\<forall>x \<in> set_btree (Node list). sep < x"
+      by fastforce
+    then have "\<forall>x \<in> set_btree_inorder (Node list). sep < x"
+      by (simp add: set_btree_inorder_set_btree)
     then have sep_sm: "\<forall>x \<in> set (inorder (Node list)). sep < x"
-      unfolding btree_set_def by auto
+      unfolding set_btree_inorder_def by auto
     then have "sorted (sep # inorder (Node list))"
       using Cons sorted_Cons_iff Cons_sorted by blast
     moreover have "\<forall>y \<in> set (inorder sub). \<forall>x \<in> set (inorder (Node list)). y < x"
       using Cons_help sep_sm pair_a Cons
-      by (metis (no_types, lifting) btree_set_def comp_apply dual_order.strict_trans list.set_intros(1) sorted_alt2.simps(2) sub_sep_cons.simps)
+      by (metis comp_apply dual_order.strict_trans list.set_intros(1) set_btree_inorder_def set_btree_inorder_set_btree sorted_alt.simps(2) sub_sep_cons.simps)
     ultimately have "sorted (inorder sub @ sep # inorder (Node list))"
       using sorted_wrt_append[of "(<)" "inorder sub" "sep # inorder (Node list)"] \<open>sorted (inorder (Node list))\<close>
-      by (metis \<open>Sorted_Less.sorted (BTree.inorder sub)\<close> btree_set_def comp_apply insert_iff list.set(2) local.Cons(2) pair_a sorted_alt2.simps(2) sub_sep_cons.simps)
+      by (metis Cons.prems(1) \<open>Sorted_Less.sorted (BTree.inorder sub)\<close> list.set_intros(1) pair_a set_btree_inorder_set_btree sorted_alt.simps(2) sorted_mid_iff sorted_pair_list sub_sep_cons.simps)
     then have "sorted ((inorder sub @ [sep]) @ inorder (Node list))"
       by simp
     then have "sorted ((\<lambda>(sub, sep). BTree.inorder sub @ [sep]) a @ foldr (@) (map (\<lambda>(sub, sep). BTree.inorder sub @ [sep]) list) [])"
@@ -420,16 +194,58 @@ proof(induction t)
   then show ?case using Node by auto
 qed auto
 
-lemma "sorted (inorder t) \<Longrightarrow> sorted_alt2 t"
+lemma sorted_inorder_subtrees: "sorted (inorder (Node xs)) \<Longrightarrow> \<forall>x \<in> set (subtrees xs). sorted (inorder x)"
+  apply(induction xs)
+  apply(auto)
+  using sorted_wrt_append apply blast
+  by (metis fst_eqD sorted_cons sorted_mid_iff)
+
+lemma sorted_inorder_subcons: "sorted (inorder (Node xs)) \<Longrightarrow> \<forall>x \<in> set xs. sub_sep_cons x"
+  apply(induction xs)
+   apply(auto)
+   apply (metis set_btree_inorder_set_btree sorted_mid_iff sorted_pair_list)
+  using sorted_cons sorted_mid_iff sorted_wrt_sorted_right by blast
+
+lemma sorted_inorder_subsepsm: "sorted (inorder (Node xs)) \<Longrightarrow> sorted_wrt sub_sep_sm xs"
+proof (induction xs)
+  case (Cons x list)
+  then obtain sub sep where x_pair: "x = (sub, sep)" by (cases x)
+  then have list_split: "inorder (Node (x#list)) = inorder sub @ sep # inorder (Node list)" unfolding inorder.simps by auto
+  then have "sorted (inorder (Node list))" 
+    using sorted_wrt_append Cons.prems sorted_cons by fastforce
+  then have sorted_wrt_rec: "sorted_wrt sub_sep_sm list" using Cons by auto
+
+  from list_split have "\<forall>l \<in> set (inorder (Node list)). sep < l"
+    by (metis Cons.prems sorted_Cons_iff sorted_wrt_append)
+  then have "\<forall>l \<in> set_btree_inorder (Node list). sep < l"
+    by (simp add: set_btree_inorder_def)
+  then have "\<forall>l \<in> set_btree (Node list). sep < l"
+    by (simp add: set_btree_inorder_set_btree)
+  then have sorted_wrt_local: "\<forall>(sub_r, sep_r) \<in> set list. (sep < sep_r \<and> (\<forall>r \<in> set_btree sub_r. sep < r))"
+    by auto
+    
+  from sorted_wrt_local sorted_wrt_rec show ?case
+    unfolding sorted_wrt.simps sub_sep_sm.simps
+    using x_pair by auto
+qed auto
+  
+
+find_theorems sorted inorder
+
+lemma sorted_sorted_alt: "sorted (inorder t) \<Longrightarrow> sorted_alt t"
 proof(induction t)
   case (Node xs)
-  then have "\<lbrakk>sorted (inorder (Node xs))\<rbrakk> \<Longrightarrow> sorted_alt2 (Node xs)"
-  proof (induction xs)
-    case (Cons a list)
-      show ?case sorry
-  qed auto
-  then show ?case using Node by auto
+  then have "\<forall>x \<in> set (subtrees xs). sorted_alt x"
+    using sorted_inorder_subtrees by fastforce
+  moreover have "\<forall>x \<in> set xs. sub_sep_cons x"
+    using Node(2) sorted_inorder_subcons by blast
+  moreover have "sorted_wrt sub_sep_sm xs"
+    using Node.prems sorted_inorder_subsepsm by blast
+  ultimately show ?case using Node by auto
 qed auto
+
+lemma sorted_alt_eq: "sorted (inorder t) = sorted_alt t"
+  using sorted_alt_sorted sorted_sorted_alt by blast
 
 
 
